<?xml version="1.0" encoding="UTF-8"?>

<section xml:id="notes-week-01">
  <title>PHY 201 Formula Sheet</title>

  <subsection xml:id="subsec-PHY-201">
    <title>PHY 201</title>

    <ul>
      <li><p><md>
 \vec{v}  = \frac{\Delta \vec{r}} {\Delta t}
 </md></p></li>
<li><p><md>
x_\mathrm{f} = x_\mathrm{i} + v_\mathrm{i} t + \tfrac{1}{2} a t^2
</md></p></li>
<li><p><md>
v_\mathrm{f} =  v_\mathrm{i} + a t
</md></p></li>
<li><p><md>
v_\mathrm{f}^2 =  v_\mathrm{i}^2 + 
2 a (x_\mathrm{f} - x_\mathrm{i})
</md></p></li>
<li><p><md>
\mean{v} =  \tfrac{1}{2} 
(v_\mathrm{f} + v_\mathrm{i}) 
</md></p></li>
\endgroup
<li><p><md>
  \Delta \vec{r}  = \mean{\vec{v}} \Delta t
</md></p></li>
<li><p><md>
\vec{F}_\mathrm{net} \equiv \sum_i \vec{F}_i
</md></p></li>
<li><p><md>
\vec{F}_\mathrm{net} = m \vec{a}
</md></p></li>
<li><p><md>
F_g = w = m g
</md></p></li>
<li><p><md>
\lvert \vec{F}_\mathrm{s} \rvert \leq \mu_\mathrm{s} \lvert \vec{n} \rvert
</md></p></li>
<li><p><md>
\lvert \vec{F}_\mathrm{k} \rvert  = \mu_\mathrm{k} \lvert \vec{n} \rvert
</md></p></li>
<li><p><md>
\vec{F}_\mathrm{S} = - k \vec{x}
</md></p></li>
<li><p><md>
\omega = \frac{v_\mathrm{t}}{r}
</md></p></li>
<li><p><md>
a_\mathrm{c} =
\frac{v_\mathrm{t}^2}{r}
= r \omega^2
</md></p></li>
<li><p><md>
F_G = G \frac{m_1 m_2}{r^2}
</md></p></li>
<li><p><md>
g = G \frac{m_\mathrm{earth}}{r^2_\mathrm{earth}}
</md></p></li>
<li><p><md>
W = \vec{F}\cdot\vec{d} 
= \lvert \vec{F} \rvert \lvert \vec{d} \rvert \cos (\theta)
</md></p></li>
<li><p><md>
P_{av}=\frac{\Delta W}{\Delta t}
</md></p></li>
<li><p><md>
\mathrm{KE} = K \equiv \tfrac{1}{2} m v^2
</md></p></li>
<li><p><md>
W_\mathrm{net} = \Delta K
</md></p></li>
<li><p><md>
W_\mathrm{cons} = -\Delta U = - \Delta \mathrm{PE}
</md></p></li>
<li><p><md>
\mathrm{PE}_g = U_g = m g h
</md></p></li>
<li><p><md>
U_G = - G \frac{m_1 m_2}{r}
</md></p></li>
<li><p><md>
\mathrm{PE}_\mathrm{S} = U_\mathrm{S} = \tfrac{1}{2} k x^2
</md></p></li>
<li><p><md>
\vec{r}_\mathrm{cm} \equiv \frac{\sum_i m_i \vec{r}_i}{\sum_i m_i}
</md></p></li>
<li><p><md>
\vec{v}_\mathrm{cm} \equiv \frac{\sum_i m_i \vec{v}_i}{\sum_i m_i}
</md></p></li>
<li><p><md>
\vec{a}_\mathrm{cm} \equiv \frac{\sum_i m_i \vec{a}_i}{\sum_i m_i}
</md></p></li>
<li><p><md>
\vec{p} \equiv m \vec{v}
</md></p></li>
<li><p><md>
\vec{F} = \frac{\Delta \vec{p}}{\Delta t}
</md></p></li>
<li><p><md>
\vec{p}_{1,\mathrm{f}} + \vec{p}_{2,\mathrm{f}} = 
\vec{p}_{1,\mathrm{i}} + \vec{p}_{2,\mathrm{i}}\; .
</md></p></li>
<li><p><md>
\vec{\mathcal{J}} \equiv \vec{F} \Delta t = \Delta \vec{p} 
</md></p></li>
%<li><p><md>
%\vec{\tau} \equiv \vec{r} \times \vec{F}
%</md></p></li>
<li><p><md>
\tau = r F \sin \theta
</md></p></li>
<li><p><md>
r_\perp = r \sin (\theta) 
</md></p></li>
<li><p><md>
\sum\tau = r_\perp F = I \alpha
</md></p></li>
%<li><p><md>
%\ell_\mathrm{in} F_\mathrm{in} = 
%\ell_\mathrm{out} F_\mathrm{out}
%</md></p></li>
<li><p><md>
  \theta =\frac{s}{r}
</md></p></li>
<li><p><md>
 \omega = \frac{\Delta \theta}{\Delta t} = \frac{v_\mathrm{t}}{r} 
</md></p></li>
<li><p><md>
 \alpha = \frac{\Delta \omega}{\Delta t} = \frac{a_\mathrm{t}}{r} 
</md></p></li>
<li><p><md>
  v = r \omega % \sin \theta
</md></p></li>
\begingroup
\allowdisplaybreaks
\abovedisplayskip=0pt
\belowdisplayskip=0pt
<li><p><md>
\theta_\mathrm{f} = \theta_\mathrm{i} + \omega_\mathrm{i} t + \tfrac{1}{2} \alpha t^2 \\
\omega_\mathrm{f} =  \omega_\mathrm{i} + \alpha t \\
\omega_\mathrm{f}^2 =  \omega_\mathrm{i}^2 + 
2 \alpha (\theta_\mathrm{f} - \theta_\mathrm{i}) \\
\mean{\omega} =  \tfrac{1}{2} 
(\omega_\mathrm{f} + \omega_\mathrm{i}) 
</md></p></li>
\endgroup
<li><p><md>
L = r p \sin \theta = I \omega
</md></p></li>
<li><p><md>
L = r (m v) \sin \theta
</md></p></li>
<li><p><md>
\vec{\tau} = \frac{\Delta \vec{L}}{\Delta t}
</md></p></li>
<li><p><md>
  W = \tau \Delta \theta 
</md></p></li>
<li><p><md>
  K_\mathrm{rot} = \tfrac{1}{2} I \omega^2
</md></p></li>
<li><p><md>
 \omega = 2 \pi f = \frac{2 \pi}{T}
</md></p></li>
<li><p><md>
 \omega = \sqrt{ \frac{k}{m} }
</md></p></li>
<li><p><md>
 \omega = \sqrt{ \frac{g}{\ell} }
</md></p></li>
<li><p><md>
 \omega = \sqrt{ \frac{m g \ell_\mathrm{cm}}{I} }
</md></p></li>
<li><p><md>
  T = 2 \pi \sqrt{ \frac{L}{g}}
</md></p></li>
<li><p><md>
  T = 2 \pi \sqrt{ \frac{I}{m g \ell_\mathrm{cm}}}
</md></p></li>
<li><p><md>
 x(t) = x_\mathrm{max} \cos (\omega t)
</md></p></li>
<li><p><md>
 v(t) = -\omega x_\mathrm{max} \sin (\omega t)
</md></p></li>
<li><p><md>
 a(t) = - \omega^2 x_\mathrm{max} \cos (\omega t)
</md></p></li>
<li><p><md>
  E = \tfrac{1}{2} k x_\mathrm{max}^2
</md></p></li>
<li><p><md>
 v = f \lambda 
</md></p></li>
<li><p><md>
  \mu \equiv \frac{m}{\ell}
</md></p></li>
<li><p><md>
  v = \sqrt{ \frac{F}{\mu} }
</md></p></li>
<li><p><md>
  k \equiv \frac{2 \pi}{\lambda}
</md></p></li>
<li><p><md>
 y_\mathrm{sw} (x,t) = \bigl [ A \sin (k x)\bigr ] \sin(\omega t)  
</md></p></li>
<li><p><md>
 f_\mathrm{string} = f_\mathrm{open-open} 
  = n \left( \frac{v}{2 \ell} \right) 
 \hspace{0.3cm}
\textnormal{where } n \in \{  1,  2, 3, \ldots \} 
</md></p></li>
<li><p><md>
 \ell = n \frac{\lambda_n}{2} 
 \hspace{0.3cm}
\textnormal{where } n \in \{  1,  2, 3, \ldots \} 
</md></p></li>
<li><p><md>
 f_\mathrm{open-closed}   = 
   n \left( \frac{v}{4 \ell} \right) 
 \hspace{0.3cm}
\textnormal{where } n \in \{  1,  3, 5, \ldots \} 
</md></p></li>
<li><p><md>
 \ell = n \frac{\lambda_n}{4}  \hspace{0.3cm}
\textnormal{where } n \in \{  1,  3, 5, \ldots \} 
</md></p></li>
<li><p><md>
 y_\mathrm{tw} (x,t) = A \sin (k x \mp \omega t)
</md></p></li>
<li><p><md>
 f_\mathrm{o} = f_\mathrm{s} 
   \left( \frac{v \pm v_\mathrm{o}}{v \mp v_\mathrm{s}} \right) 
</md></p></li>
<li><p><md>
 \Delta{L} = m\lambda 
</md></p></li>
<li><p><md>
 \Delta{L} = (m - \frac{1}{2} )\lambda 
</md></p></li>
<li><p><md>
 f_\mathrm{beat} = \lvert f_2 - f_1 \rvert 
</md></p></li>
<li><p><md>
 P = \frac{F}{A}
</md></p></li>
<li><p><md>
  \rho = \frac{m}{V}
</md></p></li>
<li><p><md>
 F_\mathrm{b} = \rho V g 
</md></p></li>
<li><p><md>
 P = P_0 + \rho g h 
</md></p></li>
<li><p><md>
 P + \rho g y + \tfrac{1}{2} \rho v^2 = \mathrm{const}
</md></p></li>
<li><p><md>
Q  = \Phi_v \equiv \vec{v}\cdot \vec{A}  = v A \cos (\theta)
</md></p></li>
<li><p><md>
Q = \frac{\Delta V}{\Delta t}
</md></p></li>
<li><p><md>
  A_1 v_1 = A_2 v_2
</md></p></li>
<li><p><md>
 \rho v A  = \frac{\Delta m}{\Delta t}
</md></p></li>
    </ul>
    
  </subsection>
  
  <subsection xml:id="subsec-Moments-of-Inertia">
    <title>Moments of Inertia</title>
    
  </subsection>
</section>
